examples/mutsum/MutGImp.v
@@ -1,0 +1,39 @@
+Require Import Coqlib.
+Require Import ITreelib.
+Require Import Universe.
+Require Import STS.
+Require Import Behavior.
+Require Import ModSem.
+Require Import Skeleton.
+Require Import PCM.
+Require Import Imp.
+
+Generalizable Variables E R A B C X Y Σ.
+
+Set Implicit Arguments.
+
+
+
+Section G.
+  Context `{Σ: GRA.t}.
+
+  Import ImpNotations.
+  Local Open Scope expr_scope.
+  Local Open Scope stmt_scope.
+
+  Definition gF :=
+    mk_function
+      ["n"]
+      (if# (Var "n")
+       then# ("f_ret" :=# (Fun "f") [(Var "n") - (Vint 1)] ;;;
+                      Expr ((Var "n") + "f_ret"))
+       else# (Expr (Vint 0)) fi#).
+
+  Definition g_prog : program :=
+    [("g", gF)].
+
+  Definition GSem: ModSem.t := ImpMod.modsem "G" g_prog.
+
+  Definition G : Mod.t := ImpMod.get_mod "G" g_prog.
+
+End G.
