examples/mutsum/MutGImp0proof.v
@@ -1,0 +1,56 @@
+Require Import HoareDef MutHeader MutGImp MutG0 SimModSem.
+Require Import Coqlib.
+Require Import Universe.
+Require Import Skeleton.
+Require Import PCM.
+Require Import ModSem Behavior.
+Require Import Relation_Definitions.
+
+(*** TODO: export these in Coqlib or Universe ***)
+Require Import Relation_Operators.
+Require Import RelationPairs.
+From ITree Require Import
+     Events.MapDefault.
+From ExtLib Require Import
+     Core.RelDec
+     Structures.Maps
+     Data.Map.FMapAList.
+
+Require Import HTactics.
+Require Import TODO.
+
+Generalizable Variables E R A B C X Y.
+
+Set Implicit Arguments.
+
+Local Open Scope nat_scope.
+
+
+
+
+Section SIMMODSEM.
+
+  Context `{Σ: GRA.t}.
+  Local Opaque GRA.to_URA.
+
+  Let W: Type := (alist mname (Σ * Any.t)) * (alist mname (Σ * Any.t)).
+
+  Let wf: W -> Prop :=
+    fun '(mrps_src0, mrps_tgt0) =>
+      (<<SRC: mrps_src0 = Maps.add "G" (ε, tt↑) Maps.empty>>) /\
+      (<<TGT: mrps_tgt0 = Maps.add "G" (ε, tt↑) Maps.empty>>)
+  .
+
+  Theorem correct: ModSemPair.sim MutG0.GSem MutGImp.GSem.
+  Proof.
+    econstructor 1 with (wf:=wf) (le:=top2); et; ss.
+    econs; ss. init. unfold cfun, gF.
+    unfold Imp.eval_function. ss. steps.
+    eapply Any.downcast_upcast in _UNWRAPN. des. clarify.
+    unfold unint in *. ss. des_ifs.
+    - steps. admit "lemmas for imp...".
+    - unfold ccall. steps.
+      admit "lemmas for imp...".
+  Qed.
+
+End SIMMODSEM.
